clos_numberProofTheory

compiler1/closLangScript.sml
@@ -1,4 +1,4 @@
-open HolKernel Parse boolLib bossLib
+open preamble;
 
 val _ = new_theory "closLang";
 
@@ -52,6 +52,105 @@ val _ = Datatype `
       | App (num option) exp (exp list)
       | Fn num (num list) num exp
       | Letrec num (num list) ((num # exp) list) exp
-      | Op op (exp list) `
+      | Op op (exp list) `;
+
+val exp_size_def = definition"exp_size_def";
+
+val code_locs_def = tDefine "code_locs" `
+  (code_locs [] = []) /\
+  (code_locs (x::y::xs) =
+     let c1 = code_locs [x] in
+     let c2 = code_locs (y::xs) in
+       c1 ++ c2) /\
+  (code_locs [Var v] = []) /\
+  (code_locs [If x1 x2 x3] =
+     let c1 = code_locs [x1] in
+     let c2 = code_locs [x2] in
+     let c3 = code_locs [x3] in
+       c1 ++ c2 ++ c3) /\
+  (code_locs [Let xs x2] =
+     let c1 = code_locs xs in
+     let c2 = code_locs [x2] in
+       c1 ++ c2) /\
+  (code_locs [Raise x1] =
+     code_locs [x1]) /\
+  (code_locs [Tick x1] =
+     code_locs [x1]) /\
+  (code_locs [Op op xs] =
+     code_locs xs) /\
+  (code_locs [App loc_opt x1 xs] =
+     let c1 = code_locs [x1] in
+     let c2 = code_locs xs in
+         c1++c2) /\
+  (code_locs [Fn loc vs num_args x1] =
+     let c1 = code_locs [x1] in
+       c1 ++ [loc]) /\
+  (code_locs [Letrec loc vs fns x1] =
+     let c1 = code_locs (MAP SND fns) in
+     let c2 = code_locs [x1] in
+     c1 ++ GENLIST ($+ loc) (LENGTH fns) ++ c2) /\
+  (code_locs [Handle x1 x2] =
+     let c1 = code_locs [x1] in
+     let c2 = code_locs [x2] in
+       c1 ++ c2) /\
+  (code_locs [Call dest xs] =
+     code_locs xs)`
+  (WF_REL_TAC `measure (exp3_size)`
+   \\ REPEAT STRIP_TAC \\ TRY DECIDE_TAC >>
+   Induct_on `fns` >>
+   srw_tac [ARITH_ss] [exp_size_def] >>
+   Cases_on `h` >>
+   fs [exp_size_def] >>
+   decide_tac);
+
+val code_locs_cons = store_thm("code_locs_cons",
+  ``∀x xs. code_locs (x::xs) = code_locs [x] ++ code_locs xs``,
+  gen_tac >> Cases >> simp[code_locs_def]);
+
+val contains_App_SOME_def = tDefine "contains_App_SOME" `
+  (contains_App_SOME [] ⇔ F) /\
+  (contains_App_SOME (x::y::xs) ⇔
+     contains_App_SOME [x] ∨
+     contains_App_SOME (y::xs)) /\
+  (contains_App_SOME [Var v] ⇔ F) /\
+  (contains_App_SOME [If x1 x2 x3] ⇔
+     contains_App_SOME [x1] ∨
+     contains_App_SOME [x2] ∨
+     contains_App_SOME [x3]) /\
+  (contains_App_SOME [Let xs x2] ⇔
+     contains_App_SOME [x2] ∨
+     contains_App_SOME xs) /\
+  (contains_App_SOME [Raise x1] ⇔
+     contains_App_SOME [x1]) /\
+  (contains_App_SOME [Tick x1] ⇔
+     contains_App_SOME [x1]) /\
+  (contains_App_SOME [Op op xs] ⇔
+     contains_App_SOME xs) /\
+  (contains_App_SOME [App loc_opt x1 x2] ⇔
+     IS_SOME loc_opt ∨ max_app < LENGTH x2 ∨
+     contains_App_SOME [x1] ∨
+     contains_App_SOME x2) /\
+  (contains_App_SOME [Fn loc vs num_args x1] ⇔
+     contains_App_SOME [x1]) /\
+  (contains_App_SOME [Letrec loc vs fns x1] ⇔
+     contains_App_SOME (MAP SND fns) ∨
+     contains_App_SOME [x1]) /\
+  (contains_App_SOME [Handle x1 x2] ⇔
+     contains_App_SOME [x1] ∨
+     contains_App_SOME [x2]) /\
+  (contains_App_SOME [Call dest xs] ⇔
+     contains_App_SOME xs)`
+  (WF_REL_TAC `measure (exp3_size)`
+   \\ REPEAT STRIP_TAC \\ TRY DECIDE_TAC >>
+   Induct_on `fns` >>
+   srw_tac [ARITH_ss] [exp_size_def] >>
+   Cases_on `h` >>
+   fs [exp_size_def] >>
+   decide_tac);
+
+val contains_App_SOME_EXISTS = store_thm("contains_App_SOME_EXISTS",
+  ``∀ls. contains_App_SOME ls ⇔ EXISTS (λx. contains_App_SOME [x]) ls``,
+  Induct >> simp[contains_App_SOME_def] >>
+  Cases_on`ls`>>fs[contains_App_SOME_def])
 
 val _ = export_theory()
