compiler1/pat_to_closScript.sml
@@ -6,7 +6,7 @@ val string_tag_def = Define`string_tag = 0:num`
 val vector_tag_def = Define`vector_tag = 1:num`
 val pat_tag_shift_def = Define`pat_tag_shift = 2:num`
 
-val _ = tDefine"compile"`
+val compile_def = tDefine"compile"`
   (compile (Raise e) =
     Raise (compile e)) ∧
   (compile (Handle e1 e2) =
@@ -178,5 +178,19 @@ val _ = tDefine"compile"`
     Cases_on`t'`>>fs[exp_size_def] >> rw[] >> simp[]
   end
 val _ = export_rewrites["compile_def"]
+
+val compile_ind = theorem"compile_ind";
+
+val compile_contains_App_SOME = store_thm("compile_contains_App_SOME",
+  ``∀e. ¬contains_App_SOME[compile e]``,
+  ho_match_mp_tac compile_ind >>
+  simp[compile_def,contains_App_SOME_def] >>
+  rw[] >> srw_tac[ETA_ss][] >>
+  rw[Once contains_App_SOME_EXISTS,EVERY_MAP] >>
+  rw[contains_App_SOME_def] >> rw[EVERY_MEM] >>
+  rw[Once contains_App_SOME_EXISTS,EVERY_MAP] >>
+  rw[contains_App_SOME_def] >> rw[EVERY_MEM] >>
+  fs[REPLICATE_GENLIST,MEM_GENLIST, MEM_MAP] >>
+  rw[contains_App_SOME_def,max_app_def]);
 
 val _ = export_theory()
